

Contents

1	Background	3
1.1	Probability vs Statistics	3
1.2	Double Integrals	3
2	Elementary (Discrete) Probability	5
2.1	Foundations	5
2.2	Conditional Probabilities	8
2.3	Independence	10
3	Discrete Random Variables	13
3.1	Random Variables	13
3.2	Discrete Random Variables	14
3.3	Discrete Distributions	16
3.4	Multiple Variables	17
3.5	Moments	18

3.6	Tails	23
4	Continuous Random Variables	24
4.1	Single Variables	24
4.2	Multiple Variables	25
4.3	Poisson Processes	25
5	(Discrete) Markov Chains	26
6	Estimators	27
6.1	Evaluation	27
6.2	Maximum Likelihood Estimation (MLE)	27

1 Background

1.1 Probability vs Statistics

- Probabilistic reasoning works forwards from a given mathematical model to the single possible prediction about given events under that model
- Statistical reasoning works backwards from given data about events to one of many possible mathematical models that could explain that data

1.2 Double Integrals

- Naive approach: Blindly compute inner then outer e.g.
$$\int_{y=0}^{y=\infty} \int_{x=0}^{x=y} e^{-y} dx dy = \int_{y=0}^{y=\infty} [xe^{-y}]_{x=0}^{x=y} dy = \int_{y=0}^{y=\infty} ye^{-y} - 0e^{-y} = \dots = 1$$

- *Fubini's Theorem:* Suppose $f(x, y)$ is continuous throughout $R = \{(x, y) \in \mathbb{R}^2 : a \leq x \leq b \text{ and } c \leq y \leq d\}$. Then, $\iint_R f(x, y) dR =$

$$\int_c^d \int_a^b f(x, y) dx dy = \int_a^b \int_c^d f(x, y) dy dx$$

- Can be easier to reverse the order as per Fubini e.g.

$$\begin{aligned} \int_{y=0}^{y=\infty} \int_{x=0}^{x=y} e^{-y} dx dy &= \int_{x=0}^{x=\infty} \int_{y=x}^{y=\infty} e^{-y} dy dx = \int_{x=0}^{x=\infty} [-e^{-y}]_{y=x}^{y=\infty} dx = \\ \int_{x=0}^{x=\infty} e^{-x} dx &= [-e^{-x}]_{x=0}^{x=\infty} = 1 \end{aligned}$$

2 Elementary (Discrete) Probability

2.1 Foundations

- All probabilities are defined based on a given experiment
- The sample space Ω = the set of possible outcomes of the experiment
- The sample space Ω is discrete iff Ω is a countable set (recall this means it may be infinite)
- The sample space Ω is continuous iff it is not discrete iff Ω is an uncountably infinite set
- An event E is $\subseteq \Omega$ i.e. zero or more outcomes
- An event is elementary iff it is singleton i.e. a single outcome

- Deduce that the set of events is closed under the standard set operations
- **Events E_1 and E_2 are mutually exclusive iff $E_1 \cap E_2 = \emptyset$**
- Recall that a family of sets (e.g events) E_1, \dots, E_n partition a set F iff $\bigcup_{i \in [n]} E_i = F$ and $\forall i \in [n]. \forall j \in [n] \setminus \{i\}. E_i \cap E_j = \emptyset$
- **The 3 axioms of probability:**
 1. **Non-negativity:** Let E be an event. Then, $P(E) \geq 0$
 2. **Additivity:** Let E_i and E_j be mutually exclusive events. Then, $P(E_i \cup E_j) = P(E_i) + P(E_j)$
 3. **Normalization:** $P(\Omega) = 1$ or equivalently $P(\emptyset) = 0$
- Note that additivity means that (by induction) the probability of any event can be broken down into a sum of probabilities of elementary events that partition it

- Proposition: $P(E \cap F) = P(E) + P(F) - P(E \cup F)$

Proof:

By additivity, $P(A) = \sum_{\omega \in A} P(\omega)$ for each A . Recall that the members of each A (the ω s) are elementary events.

Pick arbitrary $\omega \in E \cup F$. Deduce that $\omega \in E \vee \omega \in F$.

Case $\omega \in E$ but $\omega \notin F$: Then, $P(\omega)$ occurs in $P(E)$ and $P(E \cup F)$ but not in $P(F)$ and so simplifies down to $P(\omega) - P(\omega) = 0$ in $P(E) + P(F) - P(E \cup F)$

Case $\omega \in F$ but $\omega \notin E$: Then, $P(\omega)$ occurs in $P(F)$ and $P(E \cup F)$ but not in $P(E)$ and so simplifies down to $P(\omega) - P(\omega) = 0$ in $P(E) + P(F) - P(E \cup F)$

Case $\omega \in E$ and $\omega \in F$: Then, $P(\omega)$ occurs in $P(F)$ and $P(E \cup F)$ but not in $P(E)$ and so simplifies down to $P(\omega) + P(\omega) - P(\omega) = P(\omega)$ in $P(E) + P(F) - P(E \cup F)$. Moreover, $\omega \in E \cap F$.

Deduce that we have covered each term of $P(E) + P(F) - P(E \cup F)$ exactly once. Thus, we have shown that $P(E) + P(F) - P(E \cup F) = \sum_{\omega \in E \cap F} P(\omega)$ and we know that this equals $P(E \cap F)$ as required.

Corollary (**Union Bound**): $P(E \cup F) = P(E) + P(F) - P(E \cap F) \leq P(E) + P(F)$ [as $P(E \cap F) \geq 0$ by non-negativity axiom]

2.2 Conditional Probabilities

- **Probability that E occurred given that F occurred** $= P(E|F) = \frac{P(E \cap F)}{P(F)}$

Corollary: $P(E \cap F) = P(F)P(E|F) = P(E)P(F|E)$

- **Chain Rule:** Let $P(\bigcap_{i=1}^n E_i) > 0$. Then, $P(\bigcap_{i=1}^n E_i) = \prod_{i=1}^n P(E_i | \bigcap_{j=1}^{i-1} E_j)$.
For example, $P(E_1)P(E_2|E_1)P(E_3|E_1 \cap E_2)P(E_4|E_1 \cap E_2 \cap E_3) =$
 $P(E_1 \cap E_2)P(E_3|E_1 \cap E_2)P(E_4|E_1 \cap E_2 \cap E_3) =$
 $P(E_1 \cap E_2 \cap E_3)P(E_4|E_1 \cap E_2 \cap E_3) = P(E_1 \cap E_2 \cap E_3 \cap E_4)$ as claimed.
- **Theorem (Law of total probability):** Let E be an event and F_1, \dots, F_n be a partition of Ω . Then, $P(E) = \sum_{i \in [n]} P(E \cap F_i) =$

$\sum_{i \in [n]} \mathbf{P}(E|F_i)\mathbf{P}(F_i)$. For example, $\mathbf{P}(A) = \mathbf{P}(A|B) + \mathbf{P}(A|\neg B)$.

Proof: Recall that $E \subseteq \Omega$ and thus deduce that $E = E \cap \Omega$. Hence, $E = E \cap (F_1 \cup \dots \cup F_n) = E \cap F_1 \cup \dots \cup E \cap F_n$. Recall that F_1, \dots, F_n are pairwise disjoint and thus deduce that $E \cap F_1, \dots, E \cap F_n$ are pairwise disjoint. Hence, by additivity, $\mathbf{P}(A) = \mathbf{P}(A \cap B_1) + \dots + \mathbf{P}(A \cap B_n)$ as required.

- **Proposition:** Let E and F be events and G_1, \dots, G_n be a partition of Ω . Then, $\mathbf{P}(E|F) = \sum_{i \in [n]} \mathbf{P}(E|F_i \cap G_i)\mathbf{P}(F_i|G_i)$.

Proof: $\mathbf{P}(E|F) = \frac{\mathbf{P}(E \cap F)}{\mathbf{P}(F)}$. Applying law of total probability: $\mathbf{P}(E \cap F) = \sum_{i \in [n]} \mathbf{P}(E \cap F \cap G_i) = \sum_{i \in [n]} \mathbf{P}(E|F \cap G_i)\mathbf{P}(F \cap G_i) = \sum_{i \in [n]} \mathbf{P}(E|F \cap G_i)\mathbf{P}(G_i|F)\mathbf{P}(F)$. Thus, $\mathbf{P}(E|F) = \frac{\mathbf{P}(E \cap F)}{\mathbf{P}(F)} = \sum_{i \in [n]} \frac{\mathbf{P}(E|F \cap G_i)\mathbf{P}(G_i|F)\mathbf{P}(F)}{\mathbf{P}(F)} = \sum_{i \in [n]} \mathbf{P}(E|F \cap G_i)\mathbf{P}(G_i|F)$ as required.

Corollary: If $\forall i \in [n]. F \perp\!\!\!\perp G_i$, then $\mathbf{P}(E|F) = \sum_{i \in [n]} \mathbf{P}(E|F_i \cap G_i)\mathbf{P}(G_i)$; a closer symmetry with the law of total probability.

- **Theorem (Bayes' Theorem):** $P(F|E) = \frac{P(E|F)P(F)}{P(E)} = \frac{P(E|F)P(F)}{P(E|F)P(F) + P(E|\neg F)P(\neg F)}$

Proof: Recall that $P(E \cap F) = P(E|F)P(F) = P(F|E)P(E)$. Thus, $P(F|E) = \frac{P(E \cap F)}{P(E)} = \frac{P(E|F)P(F)}{P(E)}$.

By the definition of \neg , $F \cap \neg F = \emptyset$ and $F \cup \neg F = \Omega$. Hence, we can apply the law of total probability: $P(E) = P(E|F)P(F) + P(E|\neg F)P(\neg F)$ completing the proof.

2.3 Independence

- **Events A_1, \dots, A_n are independent iff $\forall S \in 2^{\{A_1, \dots, A_n\}}. P(S) = \prod_{X \in S} P(X)$.** For example, A_1, A_2, A_3, A_4 are independent iff $P(A_1 \cap A_2) = P(A_1)P(A_2)$ and $P(A_1 \cap A_3) = P(A_1)P(A_3)$ and $P(A_1 \cap A_4) = P(A_1)P(A_4)$ and $P(A_2 \cap A_3) = P(A_2)P(A_3)$ and $P(A_2 \cap A_4) = P(A_2)P(A_4)$ and $P(A_3 \cap A_4) = P(A_3)P(A_4)$ and $P(A_1 \cap A_2 \cap A_3) = P(A_1)P(A_2)P(A_3)$

and $P(A_1 \cap A_2 \cap A_4) = P(A_1)P(A_2)P(A_4)$ and $P(A_2 \cap A_3 \cap A_4) = P(A_2)P(A_3)P(A_4)$ and $P(A_1 \cap A_2 \cap A_3 \cap A_4) = P(A_1)P(A_2)P(A_3)P(A_4)$

Corollary: Events E and F are independent ($E \perp F$) iff $P(E \cap F) = P(E)P(F)$

- Proposition: Assuming that $P(E) > 0$ and $P(F) > 0$ respectively, $E \perp F$ iff $P(E|F) = P(E)$ iff $P(F|E) = P(F)$

Proof: Trivial from Bayes' theorem

- Proposition: If E_1 and E_2 are mutually exclusive events, then E_1 and E_2 are independent only if at least one of E_1 and E_2 has probability 0

Proof: E_1 and E_2 are mutually exclusive $\Rightarrow P(E_1 \cap E_2) = 0$.

E_1 and E_2 are independent $\Rightarrow P(E_1)P(E_2) = P(E_1 \cap E_2) = 0 \Rightarrow (P(E_1) = 0 \vee P(E_2) = 0)$.

- Events A_1, \dots, A_n are pairwise independent iff $\forall i \in [n]. \forall j \in [n] \setminus \{i\}. P(A_i \cap A_j) = P(A_i)P(A_j)$

- Proposition: There exists a family of events that are pairwise independent but not fully independent. Proof: Exercise
- Events E and F are conditionally independent given an event G iff $P(E \cap F|G) = P(E|G)P(F|G)$
- Proposition: There exists a family of events that are conditionally independent given some additional event but not fully independent. Proof: Exercise
- Proposition: There exists a family of events that are fully independent but for which there exists an event they are not conditionally independent given. Proof: Exercise

3 Discrete Random Variables

3.1 Random Variables

- In CS130 we only considered events: an abstraction over elementary outcomes (members of sets (or singleton sets)). In this module we focus on random variables: an abstraction over events (sets).
- A random variable X is a function $\Omega \mapsto \mathbb{R}$. Note that, unlike $P : 2^\Omega \mapsto \mathbb{R}$ which assigns a number to each set (event (collection of outcomes of experiments)), **a random variable assigns a number to each member of the set Ω (an outcome of an experiment (an elementary event))**.
- As X^{-1} assigns to each number a set of outcomes, **considering a random variable being equal to a certain value exactly corresponds to considering a certain event** ($(X = i) = \{\omega : X(\omega) = i\} = \{\omega : \omega \in X^{-1}(i)\}$)

- Proposition: $\{(X = i) : i \in \mathbb{R}\}$ is a partition of Ω .

Proof: Pick arbitrary $i \in \mathbb{R}$.

$\cup_{i \in \mathbb{R}} (X = i) = \Omega$ as $\mathbb{R} \supseteq \text{codomain}(X)$ and so this union must be the entire domain of X . (Many of the sets being unioned will be \emptyset but this is fine).

Pick arbitrary $j \in \mathbb{R}$ such that $i \neq j$. Then, $(X = i) \cap (X = j) = \emptyset$ as any element in this intersection would be an elementary outcome associated with more than one number by X and so would contradict X being a function.

3.2 Discrete Random Variables

- A discrete random variable has countable range (e.g. \mathbb{N}) whereas a continuous random variable has uncountable range (e.g. \mathbb{R}). For the rest of this chapter all random variables are discrete

- $\mathbf{p}_X(i)$ = **probability mass function (pmf) of X** = $\mathbf{P}(X = i)$
- $\mathbf{p}_{X|A}(i)$ = **probability mass function of X given A** = $\frac{\mathbf{P}(\{X=i\} \cap A)}{\mathbf{P}(A)}$. $X|A$ can be viewed as an event in its own right, with this pmf.
- $\mathbf{F}_X(i)$ = **cumulative distribution function of X** = $\mathbf{P}(X \leq i) = \mathbf{P}(\cup_{j \leq i} X = j)$ by definition = $\sum_{j \leq i} \mathbf{P}(X = j)$ by **additivity** (as the $X = j$ are a partition of $X \leq i$)
- $\neg \mathbf{F}_X(i)$ = **tail function of X** = $\mathbf{P}(X > i) = 1 - \mathbf{F}_X(i)$. Note this is not $\mathbf{P}(X \geq i)$
- Proposition: Let X be a random variable. Then, $\sum_{i \in \mathbb{R}} \mathbf{P}(X = i) = 1$
 Proof:
 i) Pick arbitrary $i \in \mathbb{R}$. Pick arbitrary $j \in \mathbb{R}$ such that $i \neq j$. Then, $(X = i) \cap (X = j) = \emptyset$ as any element in this intersection would be an elementary outcome associated with more than one number by X and so would contradict X being a function.

ii) $\cup_{i \in \mathbb{R}} (X = i) = \Omega$ as $\mathbb{R} \supseteq \text{range}(X)$ and so this union must be the entire domain of X . (Many of the sets being unioned will be \emptyset but this is fine). Combining i) and ii) $\{(X = i) : i \in \mathbb{R}\}$ is a partition of Ω . Thus, as each $X = i$ is an event, we can apply the law of total probability to obtain $\sum_{i \in \mathbb{R}} P(X = i) = P(\Omega)$. Finally, by the normalization axiom, $P(\Omega) = 1$.

3.3 Discrete Distributions

- **If $X \sim \text{Bernoulli}(p)$, then $\text{range}(X) = \{0, 1\}$ and $\mathbf{p}_X(1) = p$ and $\mathbf{p}_X(0) = 1 - p$.** Interpretation: Single trial of a binary experiment; 1 iff success; 0 iff failure; p = probability of success
- **If $X \sim \text{Binomial}(n, p)$, then $\text{range}(X) = \{0, \dots, n\}$ and $\mathbf{p}_X(i) = \binom{n}{i} (p)^i (1-p)^{n-i}$.** Interpretation: Number of successes out of n independent Bernoulli trials each with probability of success p
- **If $X \sim \text{Geometric}(p)$, then $\text{range}(X) = \mathbb{N}_{>0}$ and $\mathbf{p}_X(i) = (1-p)^{i-1}p$ and $\neg \mathbf{F}_X(i) = (1-p)^i$.** Interpretation: Number of independent Bernoulli

trials (each with probability of success p) until the first success (hence the 1 indexing as at least one trial must be required)

- **If $X \sim \text{Poisson}(\lambda)$, then $\text{range}(X) = \mathbb{N}$ and $\mathbf{p}_X(i) = e^{-\lambda} \frac{\lambda^i}{i!}$.** Interpretation: Number of events per unit time where the average number of events per unit time is λ

3.4 Multiple Variables

- **Joint probability mass function of random variables X and Y**
 $\mathbf{p}_{X,Y}(x, y) = \mathbf{P}(X = x \cap Y = y)$
- Proposition: $\mathbf{p}_X(x) = \sum_y \mathbf{p}_{X,Y}(x, y)$
 Proof: Recall that $\{Y = y\}$ is a partition of Ω .
 $\mathbf{p}_X(x) = P(X = x) = P(X = x \cap \cup_y Y = y) = P(\cup_y (X = x \cap Y = y)) = \sum_y P(X = x \cap Y = y)$ as the sets being unioned are mutually disjoint
 $= \sum_y \mathbf{p}_{X,Y}(x, y)$ by definition

- $X \perp\!\!\!\perp Y$ iff $\forall x, y. p_{X,Y}(x, y) = p_X(x)p_Y(y)$

3.5 Moments

- k^{th} moment of $X = E[X^k] = \sum_x (x^k \mathbf{P}(X = x))$

- Expectation of $X = E[X] = 1^{\text{st}}$ moment of X

- If $X \sim \text{Bernoulli}(p)$, then $E[X] = 1p + 0(1 - p) = p$

- Proposition: If $X \sim \text{Poisson}(\lambda)$, then $E[X] = \lambda$

Proof: Recall that the Maclaurin series for e^x is $\sum_{i=0}^{\infty} \frac{x^i}{i!}$.

$$E[X] = \sum_{i=0}^{\infty} i e^{-\lambda} \frac{\lambda^i}{i!} = 0 + e^{-\lambda} \sum_{i=1}^{\infty} \frac{\lambda^i}{(i-1)!} = e^{-\lambda} \lambda \sum_{i=1}^{\infty} \frac{\lambda^{i-1}}{(i-1)!} = e^{-\lambda} \lambda \sum_{i=0}^{\infty} \frac{\lambda^i}{i!} = e^{-\lambda} \lambda e^{\lambda} = \lambda.$$

- By the definition of expectation, $E[g(X)] = \sum_x (g(x) \mathbf{P}(X = x))$ and so in general $E[g(X)] \neq g(E[X])$

- **Theorem:** If $X \perp\!\!\!\perp Y$, then $E[g(X)f(Y)] = E[g(X)]E[f(Y)]$. Note that here $g(X)f(Y)$ denotes a random variable of the arithmetic product of $g(X)$ and $f(Y)$ not the Cartesian product of their distributions whereas it will be the Cartesian product in $P_{g(X)f(Y)}$.

Proof:

Lemma: $X \perp\!\!\!\perp Y \Rightarrow g(X) \perp\!\!\!\perp f(Y) \Rightarrow \forall x, y. P_{g(X)f(Y)}(x, y) = P_{g(X)}(x)P_{f(Y)}(y)$

Proof: Exercise

$$\begin{aligned} E[g(X)f(Y)] &= \sum_{x \in g(X)} \sum_{y \in f(Y)} (g(X)f(Y)P_{g(X)f(Y)}(x, y)) = \\ &= \sum_{x \in g(X)} \sum_{y \in f(Y)} (g(X)f(Y)P_{g(X)}(x)P_{f(Y)}(y)) = \\ &= \sum_{x \in g(X)} (g(x)P_{g(X)}(x)E[f(Y)]) = E[g(X)]E[f(Y)]. \end{aligned}$$

Corollary: $E[XY] = E[X]E[Y]$

- **Theorem (Linearity of expectation):** $E[g(X) + f(Y)] = E[g(X)] + E[f(Y)]$ irrespective of whether $X \perp\!\!\!\perp Y$.

$$\begin{aligned} \text{Proof: } E[g(X) + f(Y)] &= \sum_{x \in g(X)} \sum_{y \in f(Y)} ((g(X) + f(Y))P_{g(X)f(Y)}(x, y)) = \\ &= \sum_{x \in g(X)} \sum_{y \in f(Y)} (g(X)P_{g(X)f(Y)}(x, y)) + \\ &= \sum_{y \in f(Y)} \sum_{x \in g(X)} (f(Y)P_{g(X)f(Y)}(x, y)) = \end{aligned}$$

$$\sum_{x \in X} (g(X)P_X(x)) + \sum_{y \in Y} (f(Y)P_Y(y)) = E[g(X)] + E[f(Y)]$$

Corollary: $E[X + Y] = E[X] + E[Y]$

- **Proposition:** If $X \sim \text{Binomial}(n, p)$, then $E[X] = np$

Proof: Consider a family of i.i.d. random variables $Y_i \sim \text{Bernoulli}(p) \forall i \in [n]$. Deduce that then $X = \sum_{i \in [n]} Y_i$. By linearity of expectation, $E[X] = \sum_{i \in [n]} E[Y_i] = np$.

- **Theorem:** Let F_i s partition Ω . Then, $E[X] = \sum_{i \in [n]} E[X|F_i]P(F_i)$

Proof: $E[X] = \sum_{x \in X} xP_X(x) = \sum_{x \in X} x(\sum_{i \in [n]} P_{X|F_i}(x)P(F_i)) =$
 $\sum_{i \in [n]} \sum_{x \in X} xP_{X|F_i}(x)P(F_i) = \sum_{i \in [n]} P(F_i) \sum_{x \in X} xP_{X|F_i}(x) =$
 $\sum_{i \in [n]} P(F_i)E[X|F_i]$

Corollary: $E[X] = E[X|A]P(A) + E[X|\neg A]P(\neg A)$

- **Proposition:** If $X \sim \text{Geometric}(p)$, then $E[X] = \frac{1}{p}$

Proof: Consider $A =$ first trial is a failure.

Then, $E[X] = E[X|A]P(A) + E[X|\neg A]P(\neg A)$. If $\neg A$ has occurred, it has taken exactly one trial to get a success; thus $E[X|\neg A] = 1$. As trials

are independent the expected number of remaining trials after a failure is $E[X]$; thus, $E[X|A] = E[X] + 1$ as we have already had 1 trial.

Thus, $E[X] = (E[X] + 1)(1 - p) + (1)(p) = (1 - p)E[X] + 1 - p + p = E[X] - pE[X] + 1$. Thus, $pE[X] = 1$ as required.

Alternative proof: $E[X] = \sum_{i=1}^{\infty} i(1 - p)^{i-1}p = p \sum_{i=1}^{\infty} i(1 - p)^{i-1} = p \sum_{i=1}^{\infty} \frac{d}{dp}((1 - p)^i) = p \frac{d}{dp}(\sum_{i=1}^{\infty} (1 - p)^i) = p \frac{d}{dp}(\frac{1}{1 - (1 - p)}) = p \frac{d}{dp}(\frac{1}{p}) = p \frac{1}{p^2} = \frac{1}{p}$.

- Proposition: If $X \sim \text{Geometric}(p)$, then $E[X^2] = \frac{2-p}{p^2}$

Proof: Consider $A = \text{first trial is a failure}$.

Then, $E[X^2] = E[X^2|A]P(A) + E[X^2|\neg A]P(\neg A) = E[(X + 1)^2](1 - p) + 1^2p = (1 - p)[E[X^2] + 2E[X] + 1] + p = (1 - p)[E[X^2] + \frac{2+p}{p}] + p$

$pE[X^2] = \frac{2+p}{p} - \frac{p(2+p)}{p} + \frac{p(p)}{p} = \frac{2+p-2p-p^2+p^2}{p} = \frac{2-p}{p}$ as required

- $Var(X) = \text{variance of } X = E[(X - E[X])^2]$

- **Proposition:** $Var(X) = E[X^2] - E[X]^2$

Proof: $Var(X) = E[(X - E[X])^2] = E[X^2 - 2XE[X] + E[X]^2] = E[X^2] - 2E[X]E[X] + E[X]^2 = E[X^2] - 2E[X]^2 + E[X]^2 = E[X^2] - E[X]^2$

- **Proposition:** If $X \sim \text{Geometric}(p)$, then $Var(X) = \frac{1-p}{p^2}$

Proof: $Var(X) = E[X^2] - E[X]^2 = \frac{2-p}{p^2} - \left(\frac{1}{p}\right)^2 = \frac{1-p}{p^2}$

- **Theorem:** If $X \perp Y$, then $Var(X + Y) = Var(X) + Var(Y)$

Proof: $Var(X + Y) = (E[(X + Y)^2]) - (E[X + Y]^2) = (E[X^2] + 2E[XY] + E[Y^2]) - (E[X]^2 + 2E[X]E[Y] + E[Y]^2).$

As $X \perp Y$, $E[XY] = E[X]E[Y]$.

Thus, $Var(X + Y) = E[X^2] - E[X]^2 + E[Y^2] - E[Y]^2 = Var(X) + Var(Y)$
as required

Corollary: If k is a constant, then $Var(X + k) = Var(X)$

- **Proposition:** If k is a constant, then $Var(kX) = k^2 Var(X)$
 $Var(kX) = E[k^2 X^2] - E[kX]^2 = k^2 E[X^2] - k^2 E[X]^2 = k^2 Var(X)$
- **Proposition:** If $X \sim \text{Binomial}(n, p)$, then $Var(X) = np(1 - p)$
 Proof: $X = \sum_{i \in [n]} X_i$ where $X_i \sim \text{Bernoulli}(p)$.
 $Var(X_i) = E[(X_i)^2] - E[X_i]^2 = p - p^2 = p(1 - p)$.
 As X_i s are independent, $Var(X) = \sum_{i \in [n]} Var(X_i) = np(1 - p)$

3.6 Tails

4 Continuous Random Variables

4.1 Single Variables

- $p_X(i)$ = probability density function (pdf) of $X \neq P(X = i)$
- If $X \sim \text{Exp}(\lambda)$, then $\text{range}(X) = \mathbb{N}$ and $p_X(i) = \lambda e^{-\lambda i}$. Interpretation: Waiting interval between events (distributed $\text{Poisson}(\lambda)$) per unit time

4.2 Multiple Variables

4.3 Poisson Processes

5 (Discrete) Markov Chains

6 Estimators

6.1 Evaluation

6.2 Maximum Likelihood Estimation (MLE)